theories/simplang/locations.v
@@ -1,23 +1,25 @@
-From stdpp Require Import countable numbers gmap.
 From iris.prelude Require Export prelude.
 From iris.prelude Require Import options.
+From stdpp Require Import countable numbers gmap.
+(* partly adapted from lambda rust *)
 
-Record loc := { loc_car : Z }.
+Definition block := positive.
+Record loc := { loc_chunk : block; loc_idx : Z }.
 
 Global Instance loc_eq_decision : EqDecision loc.
 Proof. solve_decision. Qed.
 
-Global Instance loc_inhabited : Inhabited loc := populate {|loc_car := 0 |}.
+Global Instance loc_inhabited : Inhabited loc := populate {|loc_chunk := 1%positive; loc_idx := 0 |}.
 
 Global Instance loc_countable : Countable loc.
-Proof. by apply (inj_countable' loc_car (λ i, {| loc_car := i |})); intros []. Qed.
+Proof. by apply (inj_countable' (λ l, (loc_chunk l, loc_idx l)) (λ '(i, j), {| loc_chunk := i; loc_idx := j |})); intros []. Qed.
 
 Program Instance loc_infinite : Infinite loc :=
-  inj_infinite (λ p, {| loc_car := p |}) (λ l, Some (loc_car l)) _.
-Next Obligation. done. Qed.
+  inj_infinite (λ '(i, j), {| loc_chunk := i; loc_idx := j |}) (λ l, Some ((loc_chunk l, loc_idx l))) _.
+Next Obligation. intros []. done. Qed.
 
 Definition loc_add (l : loc) (off : Z) : loc :=
-  {| loc_car := loc_car l + off|}.
+  {| loc_chunk := loc_chunk l; loc_idx := loc_idx l + off|}.
 
 Notation "l +ₗ off" :=
   (loc_add l off) (at level 50, left associativity) : stdpp_scope.
@@ -31,16 +33,19 @@ Proof. destruct l; rewrite /loc_add /=; f_equal; lia. Qed.
 Global Instance loc_add_inj l : Inj eq eq (loc_add l).
 Proof. destruct l; rewrite /Inj /loc_add /=; intros; simplify_eq; lia. Qed.
 
-Definition fresh_locs (ls : gset loc) : loc :=
-  {| loc_car := set_fold (λ k r, (1 + loc_car k) `max` r)%Z 1%Z ls |}.
+Definition fresh_block {X} (σ : gmap loc X) : block :=
+  let loclst : list loc := elements (dom _ σ : gset loc) in
+  let blockset : gset block := foldr (λ l, ({[loc_chunk l]} ∪.)) ∅ loclst in
+  fresh blockset.
 
-Lemma fresh_locs_fresh ls i :
-  (0 ≤ i)%Z → fresh_locs ls +ₗ i ∉ ls.
+Lemma is_fresh_block {X} (σ : gmap loc X) i :
+  σ !! ({|loc_chunk := fresh_block σ; loc_idx := i |} : loc) = None.
 Proof.
-  intros Hi. cut (∀ l, l ∈ ls → loc_car l < loc_car (fresh_locs ls) + i)%Z.
-  { intros help Hf%help. simpl in *. lia. }
-  apply (set_fold_ind_L (λ r ls, ∀ l, l ∈ ls → (loc_car l < r + i)%Z));
-    set_solver by eauto with lia.
+  assert (∀ (l : loc) ls (S : gset block),
+    l ∈ ls → (loc_chunk l) ∈ foldr (λ l, ({[(loc_chunk l)]} ∪.)) S ls) as help.
+  { induction 1; set_solver. }
+  rewrite /fresh_block /= -(not_elem_of_dom (D := gset loc)) -elem_of_elements.
+  move=> /(help _ _ ∅) /=. apply is_fresh.
 Qed.
 
-Global Opaque fresh_locs.
+Global Opaque fresh_block.
